Source/DafnyCore/Verifier/Translator.ExpressionWellformed.cs
@@ -379,7 +379,7 @@ namespace Microsoft.Dafny {
               e0 = etran.TrExpr(e.E0);
               CheckWellformed(e.E0, wfOptions, locals, builder, etran);
               var f = finite ? BuiltinFunction.MapDomain : BuiltinFunction.IMapDomain;
-              Bpl.Expr inDomain = FunctionCall(selectExpr.tok, f, predef.MapType(e.tok, finite, predef.BoxType, predef.BoxType), seq);
+              Bpl.Expr inDomain = FunctionCall(selectExpr.tok, f, predef.MapType(e.tok, finite, predef.ValueType, predef.ValueType), seq);
               inDomain = Bpl.Expr.Select(inDomain, BoxIfNecessary(e.tok, e0, e.E0.Type));
               builder.Add(Assert(GetToken(expr), inDomain, new PODesc.ElementInDomain(e.Seq, e.E0), wfOptions.AssertKv));
             } else if (eSeqType is MultiSetType) {
@@ -530,10 +530,10 @@ namespace Microsoft.Dafny {
             // translate arguments to requires and reads
             Func<Expression, Bpl.Expr> TrArg = arg => {
               Bpl.Expr inner = etran.TrExpr(arg);
-              if (ModeledAsBoxType(arg.Type)) {
+              if (ModeledAsValueType(arg.Type)) {
                 return inner;
               } else {
-                return FunctionCall(arg.tok, BuiltinFunction.Box, null, inner);
+                return FunctionCall(arg.tok, null, null, inner); // todo: fix first null BuiltinFunction.Box
               }
             };
 
